make tree cursor based version of team tree

concurrency/openmp_sem/team_dyn.v
@@ -1,8 +1,102 @@
 From stdpp Require Import list.
 From mathcomp.ssreflect Require Import ssreflect ssrbool ssrfun.
 Import ListNotations.
+
+Unset Guard Checking.
+
+Section SiblingTree.
+
+  Context {B:Type}.
+  (* a tree that can have multiple children *)
+  Inductive stree :=
+  | SNode : B -> list stree -> stree.
+
+  Definition data_of (st: stree) : B :=
+    match st with | SNode b _ => b end.
+  
+  Definition kids_of (st: stree) : list stree :=
+    match st with | SNode _ kids => kids end.
+
+  Definition update_data (st: stree) (b: B) : stree :=
+    match st with | SNode _ kids => SNode b kids end.
+
+  (* stree eliminator, with the ability of knowing a node's parent
+     f (parent: option B) (current_node_info: B) (previously accumulated results: A) *)
+  Fixpoint fold_tree_p {A: Type} (st: stree) (f: option B -> B -> A -> A) (accu: A) (parent: option B) : A :=
+    match st with | SNode b kids =>
+    let accu' := f parent b accu in
+       foldr (λ st accu, fold_tree_p st f accu $ Some b) accu' kids
+    end.
+
+  Definition tree_cursor : Type := stree -> stree.
+
+  Definition tree_ref : Type := stree * tree_cursor.
+
+  (* elements to the left and to the right *)
+  Definition list_cursor {A: Type} : Type := @list A * @list A.
+
+  Definition list_ref {A: Type} : Type := A * @list_cursor A.
+
+  Definition list_cursor_kont {A: Type} (l_cursor: list_cursor) (m : A) : list A :=
+    let (l, r) := l_cursor in l ++ [m] ++ r.
+
+  Fixpoint make_list_ref_aux {A: Type} (lst: @list A) (l: @list A) : list $ @list_ref A :=
+    match lst with 
+    | m::r => (m, (l, r)) :: make_list_ref_aux r (l++[m])
+    | _ => nil
+    end.
+
+  Definition make_list_ref {A: Type} (l: @list A) : list $ @list_ref A :=
+    make_list_ref_aux l nil.
+
+  Definition kids_ref_list s (t_cursor: tree_cursor) : list tree_ref :=
+    match s with | SNode d kids =>
+      (λ l_ref, 
+      let '(kid_st, l_cursor) := l_ref in
+                                (kid_st, t_cursor ∘ (SNode d) ∘ (list_cursor_kont l_cursor))) 
+      <$> (make_list_ref kids)
+    end
+    .
+
+  Definition tree_size (s: stree) :=
+    fold_tree_p s (λ _ _ acc, 1 + acc) 0 None.
+
+  Definition tree_ref_size (ref: tree_ref) :=
+    let '(st, _) := ref in tree_size st.
+
+
+    (* probably needs to measure this; fix *)
+  Fixpoint stree_lookup_aux (is_target: stree -> bool) (ref : tree_ref) (accu: option tree_ref) {struct ref}: option tree_ref :=
+    match accu with
+    | Some _ => accu (* already found *)
+    | None =>
+      match ref with
+      | (st, cursor) =>
+      if is_target st then Some ref
+      else
+        foldr (stree_lookup_aux is_target) accu $ kids_ref_list st cursor
+      end
+    end.
+
+  Definition stree_lookup (is_target: stree -> bool) (t: stree) : option tree_ref :=
+    stree_lookup_aux is_target (t, id) None.
+
+  Lemma lookup_has_prop (is_target: stree -> bool) (t: stree) (ref: tree_ref) :
+    stree_lookup is_target t = Some ref →
+    is_target (fst ref) = true.
+  Admitted.
+
+  (* lookup with is_target, if found, update the data of the subtree root to b' *)
+  Definition stree_update (is_target: stree -> bool) (b': B) (st: stree) : option stree :=
+    ref ← stree_lookup is_target st;
+    Some (ref.2 $ update_data ref.1 b').
+
+End SiblingTree.
+
+Set Guard Checking.
+
 Section OpenMPThreads.
-    
+
     (* OpenMP thread info *)
     Record ot_info := {
       t_tid : nat; (* thread id *)
@@ -36,23 +130,17 @@ Section OpenMPThreads.
     *)
 
       (* model of the dynamics of a team. Only the leaf threads are executing, the parents are for bookkeeping. *)
-      Inductive team_tree :=
-      | TeamLeaf : ot_info -> team_tree
-      (* parent thread and the including itself *)
-      | TeamNode : ot_info -> (* parent thread *)
-                   list team_tree -> (* the team that it spawns, 
-                                        first thread is same as parent thread but o_tid=0 *)
-                   team_tree.
+      Definition team_tree := @stree ot_info.
 
       (* the first thread in the program *)
       Definition ot_init (tid: nat) := Build_ot_info tid 0 false.
 
       (* a team starts with just the main thread *)
-      Definition team_init (tid: nat) := TeamLeaf (ot_init tid).
+      Definition team_init (tid: nat) := SNode (ot_init tid) [].
 
       (* ot creates a new team with the other team_mates *)
       Definition spawn_team' (ot: ot_info) (team_mates: list nat) : team_tree :=
-        TeamNode ot $ (λ tid, TeamLeaf (Build_ot_info tid 0 false)) <$> (cons (ot.(t_tid)) team_mates).
+        SNode ot $ (λ tid, SNode (Build_ot_info tid 0 false) []) <$> (cons (ot.(t_tid)) team_mates).
 
       Definition is_tid (tid: nat) (ot: ot_info) :=
         ot.(t_tid) = tid.
@@ -62,113 +150,105 @@ Section OpenMPThreads.
       (* the list of all leaf threads *)
       Fixpoint tree_to_list (tree: team_tree) : (list ot_info) :=
         match tree with
-        | TeamLeaf ot => nil
-        | TeamNode ot ts => concat (map tree_to_list ts)
+        | SNode ot ts =>
+          match ts with
+          | [] => [ot] (* leaf node*)
+          | _ => concat (tree_to_list <$> ts)
+          end
         end.
 
-      Definition has_tid (tid: nat) (tree: team_tree) : Prop :=
-        In tid $ map t_tid $ tree_to_list tree.
+      Definition leaf_tids (t: team_tree) : list nat :=
+        t_tid <$> tree_to_list t.
 
-      Definition get_ot (tid: nat) (tree: team_tree) : option ot_info :=
-        find (λ ot, decide (ot.(t_tid) = tid)) $ tree_to_list tree.
+      Definition has_tid' (tid: nat) (tree: team_tree) : Prop :=
+        In tid $ leaf_tids tree.
+        
+      (* ot_info of the (immediate) team led by root of tree; does not include subteams *)
+      Definition team_info (tree: team_tree) : list ot_info :=
+        data_of <$> kids_of tree.
+
+      Definition has_tid (tid: nat) (tree: team_tree) : bool :=
+        isSome $ stree_lookup (λ st, decide $ is_tid tid $ data_of st) tree.
+
+      Lemma has_tid_correct tid tree :
+        has_tid tid tree = true ↔ has_tid' tid tree.
+      Proof. Admitted.
 
       Definition tid_unique (tree: team_tree) : Prop :=
-        NoDup $ map t_tid $ tree_to_list tree.
-
-      (* `tree` and `tids` contain the same tid, where `tids` is the  *)
-      Definition matching_tids (tree: team_tree) (tids: list nat) : Prop :=
-        ∀ tid, In tid tids ↔ has_tid tid tree.
+        NoDup $ t_tid <$> tree_to_list tree.
 
       Class team_tree_inv (tree: team_tree) : Prop :=
-        { inv_tid_unique    : tid_unique tree;
-          inv_matching_tids : matching_tids tree (map t_tid $ tree_to_list tree) }.
+        { inv_tid_unique    : tid_unique tree }.
 
       (** folloing opeartions assume that tids in the trees are NoDup, and the indexing tid exists as a leaf
            node in the tree. *)
       (** spawns a team at every TeamLeaf that contains tid.
        * should require that tid is unique in tree.
        *)
-      Fixpoint spawn_team (tid: nat) (team_mates: list nat) (tree: team_tree): team_tree :=
-        match tree with
-        | TeamLeaf ot => if decide $ is_tid tid ot then spawn_team' ot team_mates else tree
-        | TeamNode p ts => TeamNode p $ map (spawn_team tid team_mates) ts
+
+      (* t is a leaf node and represents tid *)
+      Definition is_leaf_tid (tid: nat) (t: team_tree) : bool :=
+        match t with
+        | SNode ot [] => decide (is_tid tid ot)
+        | _ => false
         end.
+
+      Definition lookup_tid (tid: nat) (t: team_tree) : option tree_ref :=
+        stree_lookup (is_leaf_tid tid) t.
+
+      Definition spawn_team (tid: nat) (team_mates: list nat) (tree: team_tree): option team_tree :=
+        (λ ref, ref.2 $ spawn_team' (data_of ref.1) team_mates) <$> lookup_tid tid tree.
 
       (* a spawned team is done when all team members are TeamLeaf (so don't have a working team)
          and are done *)
       Definition is_team_done (tid: nat) (tree: team_tree) : Prop :=
-        ∃ p ts,
-          tree = TeamNode p ts ∧ 
-          Forall (λ t, ∃ ot, t=TeamLeaf ot ∧ (* all team members must be leaf *)
-                             ot.(o_done) = true) ts.
+        match tree with
+        | SNode p ts => 
+          Forall (λ t, match t with SNode ot kids => (* all team members must be leaf *)
+                             ot.(o_done) = true ∧ kids = [] end) ts end.
 
+      #[global] Instance is_team_done_decidable tid tree : Decision (is_team_done tid tree).
+      Proof.
+        move : tree => [ot ts].
+        rewrite /is_team_done. apply Forall_dec => [[? ?]].
+        tc_solve.
+      Qed.
+      
       (** assume tid is the primary thread of some team, turn that TeamNode to TeamLeaf.
        * Happens when all threads, including primary, are done in this team.
       *)
-      Fixpoint fire_team (tid: nat) (tree: team_tree) : team_tree :=
+      Definition fire_team (tid: nat) (tree: team_tree) : option team_tree :=
+        (λ ref, ref.2 $ SNode (data_of ref.1) []) <$> lookup_tid tid tree.
+
+      (* whether the root of the tree is the leader of tid.
+         this requires that they are in the same team.  *)
+      Definition is_leader_tree_of (tid: nat) (tree: team_tree) : Prop :=
         match tree with
-        | TeamLeaf _ => tree
-        | TeamNode p ts => if decide $ is_tid tid p then TeamLeaf p else TeamNode p $ map (fire_team tid) ts
-        end.
-
-      Fixpoint team_tids' (trees: list team_tree) : list nat :=
-        match trees with
-        | TeamLeaf ot :: trees' => ot.(t_tid) :: team_tids' trees'
-        | TeamNode ot _ :: trees' => ot.(t_tid) :: team_tids' trees'
-        | nil => nil
-        end.
-
-      (* get all the tids of the team that is at the shallowest level of tree  *)
-      Definition team_tids (tree: team_tree) : option $ list nat :=
-        match tree with
-        | TeamLeaf _ => None
-        | TeamNode ot ts => Some $ team_tids' ts
-        end.
-
-      (* tid is in the (shallowest) team represented by tree *)
-      Definition in_team (tid: nat) (tree: team_tree) : Prop :=
-        ∃ tids, team_tids tree = Some tids ∧ In tid tids.
-
-
-      Fixpoint measure_tree (tree: team_tree) : nat :=
-        match tree with
-        | TeamLeaf _ => 1
-        | TeamNode _ ts => 1 + list_sum (map measure_tree ts)
-        end.
-
-Require Import Coq.Program.Wf.
-
-      (* FIXME this is so cursed *)
-      (* the team that contains tid *)
-       Definition is_subtree_aux (subtree: team_tree) (tree: team_tree) : Prop :=
-        subtree = tree ∨
-        ∃ ot ts, tree = TeamNode ot ts ∧
-        In subtree ts.
+        | SNode ot kids =>
+           (In tid $ t_tid <$> team_info tree) end.
       
-      (* transitive closure of is_subtree_aux *)
-      Definition is_subtree (subtree: team_tree) (tree: team_tree) : Prop :=
-        is_subtree_aux subtree tree ∨ ∃ sub', is_subtree_aux subtree sub' ∧ is_subtree_aux sub' tree.
+      #[global] Instance is_leader_tree_of_dec tid tree : Decision (is_leader_tree_of tid tree).
+      Proof.
+        move : tree => [ot ts].
+        rewrite /is_leader_tree_of.
+        apply In_dec => [? ?]. apply Nat.eq_dec.
+      Qed.
 
-      (* find the leader's tid for input tid *)
-      Definition leader_tid (tid: nat) (tree: team_tree) (leader_tid: nat) : Prop :=
-        ∃ subtree ot_leader ts,
-          is_subtree subtree tree ∧
-          subtree = TeamNode ot_leader ts ∧
-          is_tid leader_tid ot_leader ∧
-          in_team tid subtree.
+      Definition leader_tree_of (tid: nat) (tree: team_tree) : option tree_ref :=
+        stree_lookup (λ st, decide $ is_leader_tree_of tid st) tree.
 
-      (* TODO make a tree_map? *)
-      (* set the tid to be done in its current parallel scope;
-         i.e. only the ot_info in the TeamLeaf that contains tid *)
-      Fixpoint set_tid_done (tid: nat) (tree: team_tree) : team_tree :=
-        match tree with
-        | TeamLeaf ot => 
-          if decide (is_tid tid ot)
-          then TeamLeaf $ Build_ot_info ot.(t_tid) ot.(o_team_id) true 
-          else TeamLeaf ot
-        | TeamNode ot ts => TeamNode ot $ map (set_tid_done tid) ts
-        end.
+      Lemma has_leader_or_no_kid (tid: nat) (tree: team_tree) :
+        has_tid tid tree ->
+        ¬(kids_of tree = []) ->
+        ∃ leader_tree,  leader_tree_of tid tree = Some leader_tree.
+      Proof. Admitted.
+
+      Definition set_tid_done (tid: nat) (tree: team_tree) : option team_tree :=
+        ref ← lookup_tid tid tree;
+        let ot := data_of ref.1 in
+        let kids := kids_of ref.1 in
+        Some (ref.2 $ SNode (Build_ot_info ot.(t_tid) ot.(o_team_id) true) kids).
 
     End OpenMPTeam.
-
+    
 End OpenMPThreads.
